PAC_Checker_LLVM/LLVM_String.thy
@@ -38,6 +38,54 @@ sepref_register \<open>(\<le>) :: char list \<Rightarrow> char list \<Rightarrow
 lemmas strl_less_hnr[sepref_fr_rules] = strl.cl_less_hnr[unfolded list_lt_less]
 lemmas strl_le_hnr[sepref_fr_rules] = strl.cl_le_hnr[unfolded list_le_less_eq]
 
+text \<open>A Hash function for Strings\<close>
+
+definition \<open>fnv1a_of_strl \<equiv> 
+  foldl (\<lambda>acc x. (acc XOR w64_of_char x) * fnv_prime) fnv_offset\<close>
+
+definition \<open>fnv1a_of_strl_inner \<equiv> \<lambda>acc x. (acc XOR w64_of_char x) * fnv_prime\<close>
+
+sepref_def fnv1a_of_strl_inner_impl is \<open>uncurry (RETURN oo fnv1a_of_strl_inner)\<close>
+  :: \<open>(word_assn' TYPE(64))\<^sup>k *\<^sub>a char_assn\<^sup>k \<rightarrow>\<^sub>a (word_assn' TYPE(64))\<close>
+  unfolding fnv1a_of_strl_inner_def
+  by sepref
+
+lemma fnv1a_of_strl_inner_rule: \<open>llvm_htriple
+  ((word_assn' TYPE(64)) w wi ** char_assn c ci)
+  (fnv1a_of_strl_inner_impl wi ci)
+  (\<lambda>r. word_assn (fnv1a_of_strl_inner w c) r ** char_assn c ci)\<close>
+  supply [vcg_rules] = hfref_htriple_k2[OF fnv1a_of_strl_inner_impl.refine]
+  apply vcg
+  by (auto simp: ENTAILS_def entails_def sep_algebra_simps pure_def)
+  
+definition \<open>fnv1a_of_strl_impl xs \<equiv> cl_fold fnv1a_of_strl_inner_impl (xs, fnv_offset)\<close>
+
+lemma fnv1a_of_strl_comp: \<open>fnv1a_of_strl = foldl fnv1a_of_strl_inner fnv_offset\<close>
+  unfolding fnv1a_of_strl_def fnv1a_of_strl_inner_def by simp
+
+lemma fnv1a_of_strl_inner_rule':
+  \<open>llvm_htriple
+    (\<up>(wi = w) ** char_assn c ci)
+    (fnv1a_of_strl_inner_impl wi ci)
+    (\<lambda>r. \<up>(r = fnv1a_of_strl_inner w c) ** char_assn c ci)\<close>
+  using fnv1a_of_strl_inner_rule[of w wi c ci]
+  by (simp add: pure_def)
+
+lemmas fnv1a_of_strl_walk_rule =
+  cl_fold_rule[where R = \<open>\<lambda>a c. \<up>(c = a)\<close> and A = \<open>char_assn\<close>
+    and f = \<open>fnv1a_of_strl_inner_impl\<close> and fa = \<open>fnv1a_of_strl_inner\<close>,
+    OF fnv1a_of_strl_inner_rule']
+
+sepref_register fnv1a_of_strl
+
+lemma fnv1a_of_strl_hnr[sepref_fr_rules]:
+  \<open>(fnv1a_of_strl_impl, RETURN o fnv1a_of_strl) \<in> strl_assn'\<^sup>k \<rightarrow>\<^sub>a (word_assn' TYPE(64))\<close>
+  unfolding fnv1a_of_strl_impl_def
+  apply sepref_to_hoare
+  supply [vcg_rules] = fnv1a_of_strl_walk_rule
+  supply [simp] = fnv1a_of_strl_comp
+  by vcg
+
 experiment
 begin
 
